BlockCacheSystem/JournalDiskUtils.i.dfy
@@ -1,5 +1,6 @@
 include "DiskLayout.i.dfy"
 include "AsyncSectorDiskModel.i.dfy"
+include "../lib/Base/sequences.i.dfy"
 
 module JournalDiskUtils {
   import opened DiskLayout
@@ -9,6 +10,7 @@ module JournalDiskUtils {
   import opened AsyncSectorDisk
   import opened Journal
   import opened Options
+  import opened Sequences
 
   type DiskConstants = AsyncSectorDisk.Constants
   type DiskState = AsyncSectorDisk.Variables
@@ -19,32 +21,132 @@ module JournalDiskUtils {
     && 0 <= len <= NumJournalBlocks() as int
   }
 
+  predicate NoOverlaps(reqWrites: map<ReqId, ReqWrite>)
+  {
+    forall id1, id2 | id1 in reqWrites && id2 in reqWrites ::
+        !overlap(reqWrites[id1].loc, reqWrites[id2].loc)
+  }
+
+  function Disk_JournalBlockAtLoc(blocks: imap<Location, Sector>, loc: Location)
+    : Option<JournalRange>
+  {
+    if loc in blocks && blocks[loc].SectorJournal? then
+      Some(blocks[loc].journal)
+    else
+      None
+  }
+
+  function Disk_JournalBlockAt(blocks: imap<Location, Sector>, i: int)
+    : Option<JournalRange>
+  requires 0 <= i < NumJournalBlocks() as int
+  {
+    Disk_JournalBlockAtLoc(blocks, JournalRangeLocation(i as uint64, 1))
+  }
+
+  function Queue_JournalBlockAt(reqWrites: map<ReqId, ReqWrite>, i: int)
+    : Option<JournalRange>
+  requires 0 <= i < NumJournalBlocks() as int
+  {
+    var loc := JournalRangeLocation(i as uint64, 1);
+    if id :| id in reqWrites
+        && ValidJournalLocation(reqWrites[id].loc)
+        && LocationSub(loc, reqWrites[id].loc) then (
+      if reqWrites[id].sector.SectorJournal?
+         && 0 <= i - JournalBlockIdx(reqWrites[id].loc) < 
+            JournalRangeLen(reqWrites[id].sector.journal) then (
+        Some(JournalBlockGet(reqWrites[id].sector.journal,
+            i - JournalBlockIdx(reqWrites[id].loc)))
+      ) else (
+        None
+      )
+    ) else (
+      None
+    )
+  }
+
+  function DiskQueue_JournalBlockAt(disk: DiskState, i: int)
+    : Option<JournalRange>
+  requires 0 <= i < NumJournalBlocks() as int
+  {
+    if Queue_JournalBlockAt(disk.reqWrites, i).Some? then
+      Queue_JournalBlockAt(disk.reqWrites, i)
+    else
+      Disk_JournalBlockAt(disk.blocks, i)
+  }
+
+  function Disk_JournalBlockSeq_i(blocks: imap<Location, Sector>, i: int)
+    : (res : seq<Option<JournalRange>>)
+  requires 0 <= i <= NumJournalBlocks() as int
+  ensures |res| == i
+  ensures forall j | 0 <= j < i :: res[j] == Disk_JournalBlockAt(blocks, j)
+  {
+    if i == 0 then [] else
+      Disk_JournalBlockSeq_i(blocks, i-1) + [Disk_JournalBlockAt(blocks, i-1)]
+  }
+
+  function Disk_JournalBlockSeq(blocks: imap<Location, Sector>)
+    : (res : seq<Option<JournalRange>>)
+  ensures |res| == NumJournalBlocks() as int
+  ensures forall j | 0 <= j < NumJournalBlocks() as int :: res[j] == Disk_JournalBlockAt(blocks, j)
+  {
+    Disk_JournalBlockSeq_i(blocks, NumJournalBlocks() as int)
+  }
+
+  function DiskQueue_JournalBlockSeq_i(disk: DiskState, i: int)
+    : (res : seq<Option<JournalRange>>)
+  requires 0 <= i <= NumJournalBlocks() as int
+  ensures |res| == i
+  ensures forall j | 0 <= j < i :: res[j] == DiskQueue_JournalBlockAt(disk, j)
+  {
+    if i == 0 then [] else
+      DiskQueue_JournalBlockSeq_i(disk, i-1) + [DiskQueue_JournalBlockAt(disk, i-1)]
+  }
+
+  function DiskQueue_JournalBlockSeq(disk: DiskState)
+    : (res : seq<Option<JournalRange>>)
+  ensures |res| == NumJournalBlocks() as int
+  ensures forall j | 0 <= j < NumJournalBlocks() as int :: res[j] == DiskQueue_JournalBlockAt(disk, j)
+  {
+    DiskQueue_JournalBlockSeq_i(disk, NumJournalBlocks() as int)
+  }
+
+  function CyclicSlice<T>(s: seq<T>, start: int, len: int) : seq<T>
+  requires |s| == NumJournalBlocks() as int
+  requires 0 <= start < NumJournalBlocks() as int
+  requires 0 <= len <= NumJournalBlocks() as int
+  {
+    if start + len <= NumJournalBlocks() as int then
+      s[start .. start + len]
+    else
+      s[start ..] + s[.. start + len - NumJournalBlocks() as int]
+  }
+
+  predicate fullRange(s: seq<Option<JournalRange>>)
+  {
+    forall i | 0 <= i < |s| :: s[i].Some?
+  }
+
+  function concatFold(s: seq<Option<JournalRange>>) : JournalRange
+  requires fullRange(s)
+  {
+    if s == [] then JournalRangeEmpty() else
+      JournalRangeConcat(concatFold(DropLast(s)), Last(s).value)
+  }
+
   predicate Disk_HasJournalRange(
       blocks: imap<Location, Sector>, start: int, len: int)
   requires WFRange(start, len)
   {
-    && (JournalFrontLocation(start as uint64, len as uint64).Some? ==>
-      && JournalFrontLocation(start as uint64, len as uint64).value in blocks
-      && blocks[JournalFrontLocation(start as uint64, len as uint64).value].SectorJournal?
-    )
-    && (JournalBackLocation(start as uint64, len as uint64).Some? ==>
-      && JournalBackLocation(start as uint64, len as uint64).value in blocks
-      && blocks[JournalBackLocation(start as uint64, len as uint64).value].SectorJournal?
-    )
+    && var slice := CyclicSlice(Disk_JournalBlockSeq(blocks), start, len);
+    && fullRange(slice)
   }
 
   function Disk_JournalRange(blocks: imap<Location, Sector>, start: int, len: int) : JournalRange
   requires WFRange(start, len)
   requires Disk_HasJournalRange(blocks, start, len)
   {
-    if JournalBackLocation(start as uint64, len as uint64).Some? then
-      JournalRangeConcat(
-          blocks[JournalFrontLocation(start as uint64, len as uint64).value].journal,
-          blocks[JournalBackLocation(start as uint64, len as uint64).value].journal)
-    else if JournalFrontLocation(start as uint64, len as uint64).Some? then
-      blocks[JournalFrontLocation(start as uint64, len as uint64).value].journal
-    else
-      JournalRangeEmpty()
+    var slice := CyclicSlice(Disk_JournalBlockSeq(blocks), start, len);
+    concatFold(slice)
   }
 
   protected predicate Disk_HasJournal(
@@ -63,116 +165,175 @@ module JournalDiskUtils {
     parseJournalRange(Disk_JournalRange(blocks, start, len)).value
   }
 
-  predicate NoOverlaps(reqWrites: map<ReqId, ReqWrite>)
-  {
-    forall id1, id2 | id1 in reqWrites && id2 in reqWrites ::
-        !overlap(reqWrites[id1.loc], reqWrites[id2.loc])
-  }
-
-  function Disk_JournalBlockAtLoc(blocks: imap<Location, Sector>, loc: Location)
-    : Option<JournalRange>
-  {
-    if loc in blocks && blocks[loc].SectorJournal? then
-      Some(blocks[loc].journal)
-    else
-      None
-  }
-
-  function Disk_JournalBlockAt(blocks: imap<Location, Sector>, i: int)
-    : Option<JournalRange>
-  requires 0 <= i < NumJournalBlocks()
-  {
-    Disk_JournalBlockAtLoc(blocks, JournalRangeLocation(i, 1))
-  }
-
-  function Queue_JournalBlockAt(reqWrites: map<ReqId, ReqWrite>, i: int)
-    : Option<JournalRange>
-  requires 0 <= i < NumJournalBlocks()
-  {
-    var loc := JournalRangeLocation(i, 1);
-    if id :| id in reqWrites && LocationSub(loc, reqWrites[id].loc) then (
-      if reqWrites[loc].sector.SectorJournal?
-         && 0 <= i - JournalBlockIdx(reqWrites[id].loc) < 
-            JournalRangeLen(reqWrites[loc].sector.journal) then (
-        Some(JournalBlockGet(reqWrites[loc].sector.journal,
-            i - JournalBlockIdx(reqWrites[id].loc)))
-      ) else (
-        None
-      )
-    ) else (
-      None
-    )
-  }
-
-  function DiskQueue_JournalBlockAt(disk: DiskState, i: int)
-    : Option<JournalRange>
-  requires 0 <= i < NumJournalBlocks()
-  {
-    if Queue_JournalBlockAt(disk.reqWrites, i).Some? then
-      Queue_JournalBlockAt(disk.reqWrites, i)
-    else
-      Disk_JournalBlockAt(disk.blocks, i)
-  }
-
-  function DiskQueue_JournalBlockSeq_i(disk: DiskState, i: int)
-    : (res : seq<Option<JournalRange>>)
-  requires 0 <= i <= NumJournalBlocks()
-  ensures |res| == i
-  ensures forall j | 0 <= j < i :: res[j] == DiskQueue_JournalBlockAt(disk, j)
-  {
-    if i == 0 then [] else
-      Disk_JournalBlockSeq_i(disk, i-1) + [DiskQueue_JournalBlockAt(disk, i-1)]
-  }
-
-  function DiskQueue_JournalBlockSeq(disk: DiskState)
-  ensures forall j | 0 <= j < NumJournalBlocks() :: res[j] == DiskQueue_JournalBlockAt(disk, j)
-  {
-    Disk_JournalBlockSeq_i(disk, NumJournalBlocks())
-  }
-
   predicate DiskQueue_HasJournalRange(
       disk: DiskState, start: int, len: int)
   requires WFRange(start, len)
   {
-    NoOverlapsInRange(disk.reqWrites, 
+    && NoOverlaps(disk.reqWrites)
+    && var slice := CyclicSlice(DiskQueue_JournalBlockSeq(disk), start, len);
+    && fullRange(slice)
   }
 
   function DiskQueue_JournalRange(
       disk: DiskState, start: int, len: int) : JournalRange
   requires WFRange(start, len)
-  requires DiskQueue_HasJournal(disk, start, len)
-
-
-
+  requires DiskQueue_HasJournalRange(disk, start, len)
+  {
+    var slice := CyclicSlice(DiskQueue_JournalBlockSeq(disk), start, len);
+    concatFold(slice)
+  }
 
   protected predicate DiskQueue_HasJournal(
       disk: DiskState, start: int, len: int)
   requires WFRange(start, len)
+  {
+    && DiskQueue_HasJournalRange(disk, start, len)
+    && parseJournalRange(DiskQueue_JournalRange(disk, start, len)).Some?
+  }
 
   protected function DiskQueue_Journal(
       disk: DiskState, start: int, len: int) : seq<JournalEntry>
   requires WFRange(start, len)
   requires DiskQueue_HasJournal(disk, start, len)
+  {
+    parseJournalRange(DiskQueue_JournalRange(disk, start, len)).value
+  }
 
   lemma Disk_eq_DiskQueue(disk: DiskState, start: int, len: int)
   requires WFRange(start, len)
-  requires Disk_HasJournal(disk.blocks, start, len)
+  requires DiskQueue_HasJournal(disk, start, len)
   requires forall id | id in disk.reqWrites ::
       locDisjointFromCircularJournalRange(
           disk.reqWrites[id].loc, start as uint64, len as uint64)
-  ensures DiskQueue_HasJournal(disk, start, len)
+  ensures Disk_HasJournal(disk.blocks, start, len)
   ensures Disk_Journal(disk.blocks, start, len)
       == DiskQueue_Journal(disk, start, len)
+  {
+    var dq := DiskQueue_JournalBlockSeq(disk);
+    var d := Disk_JournalBlockSeq(disk.blocks);
+    var dq_slice := CyclicSlice(dq, start, len);
+    var d_slice := CyclicSlice(d, start, len);
+    assert |d_slice| == |dq_slice|;
+    forall i | 0 <= i < |d_slice|
+    ensures d_slice[i] == dq_slice[i]
+    {
+      var j := JournalPosAdd(start, i);
+      calc {
+        d_slice[i];
+        d[j];
+        dq[j];
+        dq_slice[i];
+      }
+    }
+    assert d_slice == dq_slice;
+  }
 
   lemma Disk_Journal_empty(disk: DiskState, start: int)
   requires WFRange(start, 0)
   ensures Disk_HasJournal(disk.blocks, start, 0)
   ensures Disk_Journal(disk.blocks, start, 0) == []
+  {
+    assert CyclicSlice(Disk_JournalBlockSeq(disk.blocks), start, 0)
+        == [];
+    assert Disk_JournalRange(disk.blocks, start, 0)
+        == JournalRangeEmpty();
+    parseJournalRangeEmpty();
+  }
 
   lemma DiskQueue_Journal_empty(disk: DiskState, start: int)
   requires WFRange(start, 0)
+  requires NoOverlaps(disk.reqWrites)
   ensures DiskQueue_HasJournal(disk, start, 0)
   ensures DiskQueue_Journal(disk, start, 0) == []
+  {
+    assert CyclicSlice(DiskQueue_JournalBlockSeq(disk), start, 0)
+        == [];
+    parseJournalRangeEmpty();
+    assert DiskQueue_JournalRange(disk, start, 0)
+        == JournalRangeEmpty();
+  }
+
+  function mapSome<T>(s: seq<T>) : (res : seq<Option<T>>)
+  ensures |res| == |s|
+  ensures forall i | 0 <= i < |res| :: res[i] == Some(s[i])
+  {
+    if s == [] then [] else mapSome(DropLast(s)) + [Some(Last(s))]
+  }
+
+  lemma concatFold_mapSome_JournalBlocks_eq_self(jr: JournalRange)
+  ensures concatFold(mapSome(JournalBlocks(jr))) == jr
+  {
+    assume false;
+  }
+
+  lemma concatFoldAdditive(
+      a: seq<Option<JournalRange>>,
+      b: seq<Option<JournalRange>>)
+  requires fullRange(a)
+  requires fullRange(b)
+  ensures fullRange(a + b)
+  ensures concatFold(a + b)
+      == JournalRangeConcat(concatFold(a), concatFold(b))
+  {
+    if |b| == 0 {
+      assert b == [];
+      assert a + b == a;
+      calc {
+        concatFold(a + b);
+        concatFold(a);
+        {
+          JournalRangeConcatEmpty(concatFold(a));
+        }
+        JournalRangeConcat(concatFold(a), JournalRangeEmpty());
+        JournalRangeConcat(concatFold(a), concatFold(b));
+      }
+    } else {
+      concatFoldAdditive(a, b[..|b|-1]);
+      assert (a + b)[..|a+b|-1] == a + b[..|b|-1];
+      assert (a+b)[|a+b|-1] == b[|b|-1];
+      JournalRangeConcatAssoc(concatFold(a), concatFold(b[..|b|-1]), b[|b|-1].value);
+      calc {
+        concatFold(a + b);
+        JournalRangeConcat(concatFold((a + b)[..|a+b|-1]), (a+b)[|a+b|-1].value);
+        JournalRangeConcat(concatFold(a + b[..|b|-1]), b[|b|-1].value);
+        JournalRangeConcat(JournalRangeConcat(concatFold(a), concatFold(b[..|b|-1])), b[|b|-1].value);
+        JournalRangeConcat(concatFold(a), JournalRangeConcat(concatFold(b[..|b|-1]), b[|b|-1].value));
+        JournalRangeConcat(concatFold(a), concatFold(b));
+      }
+    }
+  }
+
+  lemma DiskQueue_Journal_append_other(
+      k: DiskConstants, disk: DiskState, disk': DiskState,
+      start: int, len: int, dop: DiskOp)
+  requires WFRange(start, len)
+  requires AsyncSectorDisk.RecvWrite(k, disk, disk', dop)
+  requires !dop.reqWrite.sector.SectorJournal?
+  requires DiskQueue_HasJournal(disk, start, len)
+  requires NoOverlaps(disk'.reqWrites)
+  ensures DiskQueue_HasJournal(disk', start, len)
+  ensures DiskQueue_Journal(disk', start, len)
+      == DiskQueue_Journal(disk, start, len)
+  {
+    var dq := DiskQueue_JournalBlockSeq(disk);
+    var dq' := DiskQueue_JournalBlockSeq(disk');
+
+    var slice := CyclicSlice(dq, start, len);
+    var slice' := CyclicSlice(dq', start, len);
+
+    assert |slice'| == |slice|;
+    forall i | 0 <= i < |slice'| ensures slice'[i] == slice[i]
+    {
+      var j := JournalPosAdd(start, i);
+      calc {
+        slice'[i];
+        dq'[j];
+        dq[j];
+        slice[i];
+      }
+    }
+    assert slice' == slice;
+  }
 
   lemma DiskQueue_Journal_append(
       k: DiskConstants, disk: DiskState, disk': DiskState,
@@ -180,13 +341,188 @@ module JournalDiskUtils {
       dop: DiskOp)
   requires WFRange(start, len)
   requires AsyncSectorDisk.RecvWrite(k, disk, disk', dop)
+  requires dop.reqWrite.sector == SectorJournal(jr)
   requires DiskQueue_HasJournal(disk, start, len)
   requires parseJournalRange(jr).Some?
   requires len + JournalRangeLen(jr) <= NumJournalBlocks() as int
   requires JournalPosAdd(start, len) + JournalRangeLen(jr) <= NumJournalBlocks() as int
+  requires NoOverlaps(disk'.reqWrites)
+  requires dop.reqWrite.loc == JournalRangeLocation(
+      JournalPosAdd(start, len) as uint64,
+      JournalRangeLen(jr) as uint64)
   ensures DiskQueue_HasJournal(disk', start, len + JournalRangeLen(jr))
   ensures DiskQueue_Journal(disk', start, len + JournalRangeLen(jr))
       == DiskQueue_Journal(disk, start, len) + parseJournalRange(jr).value
+  {
+    var dq := DiskQueue_JournalBlockSeq(disk);
+    var dq' := DiskQueue_JournalBlockSeq(disk');
+
+    var slice := CyclicSlice(dq, start, len);
+    var slice_jr := slice + mapSome(JournalBlocks(jr));
+
+    var slice' := CyclicSlice(dq', start, len + JournalRangeLen(jr));
+
+    assert |slice'| == |slice_jr|;
+    forall i | 0 <= i < |slice'| ensures slice'[i] == slice_jr[i]
+    {
+      var j := JournalPosAdd(start, i);
+      if i < len {
+        calc {
+          slice'[i];
+          dq'[j];
+          dq[j];
+          slice_jr[i];
+        }
+      } else {
+        //assert 0 <= i - len;
+        //assert i - len <= JournalRangeLen(jr);
+
+        var loc := JournalRangeLocation(j as uint64, 1);
+        assert dop.id in disk'.reqWrites;
+        assert ValidJournalLocation(disk'.reqWrites[dop.id].loc);
+        assert LocationSub(loc, disk'.reqWrites[dop.id].loc);
+        assert disk'.reqWrites[dop.id].sector.SectorJournal?;
+        assert 0 <= j - JournalBlockIdx(disk'.reqWrites[dop.id].loc) < 
+            JournalRangeLen(disk'.reqWrites[dop.id].sector.journal);
+
+        assert Queue_JournalBlockAt(disk'.reqWrites, j).Some?;
+        calc {
+          slice'[i];
+          dq'[j];
+          DiskQueue_JournalBlockAt(disk', j);
+          Queue_JournalBlockAt(disk'.reqWrites, j);
+          Some(JournalBlockGet(jr, i - len));
+          slice_jr[i];
+        }
+      }
+    }
+    assert slice' == slice_jr;
+
+    calc {
+      concatFold(slice');
+      concatFold(slice_jr);
+      {
+        concatFoldAdditive(slice, mapSome(JournalBlocks(jr)));
+      }
+      JournalRangeConcat(concatFold(slice),
+            concatFold(mapSome(JournalBlocks(jr))));
+      {
+        concatFold_mapSome_JournalBlocks_eq_self(jr);
+      }
+      JournalRangeConcat(concatFold(slice), jr);
+    }
+
+    parseJournalRangeAdditive(concatFold(slice), jr);
+  }
+
+  lemma DiskQueue_Journal_append_wraparound(
+      k: DiskConstants, disk: DiskState, disk': DiskState,
+      start: int, len: int, jr: JournalRange,
+      dop: DiskOp)
+  requires WFRange(start, len)
+  requires AsyncSectorDisk.RecvWrite2(k, disk, disk', dop)
+  requires len + JournalRangeLen(jr) <= NumJournalBlocks() as int
+  requires JournalPosAdd(start, len) + JournalRangeLen(jr) >= NumJournalBlocks() as int
+  requires dop.reqWrite1.sector == SectorJournal(JournalRangePrefix(jr, NumJournalBlocks() as int - start - len))
+  requires dop.reqWrite2.sector == SectorJournal(JournalRangeSuffix(jr, NumJournalBlocks() as int - start - len))
+  requires DiskQueue_HasJournal(disk, start, len)
+  requires parseJournalRange(jr).Some?
+  requires NoOverlaps(disk'.reqWrites)
+  requires dop.reqWrite1.loc == JournalRangeLocation(
+      JournalPosAdd(start, len) as uint64,
+      (NumJournalBlocks() - start as uint64 - len as uint64))
+  requires dop.reqWrite2.loc == JournalRangeLocation(
+      0,
+      JournalRangeLen(jr) as uint64 - (NumJournalBlocks() - start as uint64 - len as uint64))
+  ensures DiskQueue_HasJournal(disk', start, len + JournalRangeLen(jr))
+  ensures DiskQueue_Journal(disk', start, len + JournalRangeLen(jr))
+      == DiskQueue_Journal(disk, start, len) + parseJournalRange(jr).value
+  {
+    var dq := DiskQueue_JournalBlockSeq(disk);
+    var dq' := DiskQueue_JournalBlockSeq(disk');
+
+    var jr1 := JournalRangePrefix(jr, NumJournalBlocks() as int - start - len);
+    var jr2 := JournalRangeSuffix(jr, NumJournalBlocks() as int - start - len);
+    var len1 := NumJournalBlocks() as int - start - len;
+
+    var slice := CyclicSlice(dq, start, len);
+    var slice_jr := slice + mapSome(JournalBlocks(jr));
+
+    var slice' := CyclicSlice(dq', start, len + JournalRangeLen(jr));
+
+    assert |slice'| == |slice_jr|;
+    forall i | 0 <= i < |slice'| ensures slice'[i] == slice_jr[i]
+    {
+      var j := JournalPosAdd(start, i);
+      if i < len {
+        calc {
+          slice'[i];
+          dq'[j];
+          dq[j];
+          slice_jr[i];
+        }
+      } else if i < len + len1 {
+        assert 0 <= i - len;
+        assert i - len <= JournalRangeLen(jr);
+
+        var loc := JournalRangeLocation(j as uint64, 1);
+        assert dop.id1 in disk'.reqWrites;
+        assert ValidJournalLocation(disk'.reqWrites[dop.id1].loc);
+        assert LocationSub(loc, disk'.reqWrites[dop.id1].loc);
+        assert disk'.reqWrites[dop.id1].sector.SectorJournal?;
+        assert 0 <= j - JournalBlockIdx(disk'.reqWrites[dop.id1].loc) < 
+            JournalRangeLen(disk'.reqWrites[dop.id1].sector.journal);
+
+        assert Queue_JournalBlockAt(disk'.reqWrites, j).Some?;
+        calc {
+          slice'[i];
+          dq'[j];
+          DiskQueue_JournalBlockAt(disk', j);
+          Queue_JournalBlockAt(disk'.reqWrites, j);
+          Some(JournalBlockGet(jr1, i - len));
+          slice_jr[i];
+        }
+      } else {
+        assert 0 <= i - len;
+        assert i - len <= JournalRangeLen(jr);
+
+        var loc := JournalRangeLocation(j as uint64, 1);
+        assert dop.id2 in disk'.reqWrites;
+        assert ValidJournalLocation(disk'.reqWrites[dop.id2].loc);
+        assert LocationSub(loc, disk'.reqWrites[dop.id2].loc);
+        assert disk'.reqWrites[dop.id2].sector.SectorJournal?;
+        assert 0 <= j - JournalBlockIdx(disk'.reqWrites[dop.id2].loc) < 
+            JournalRangeLen(disk'.reqWrites[dop.id2].sector.journal);
+
+        assert Queue_JournalBlockAt(disk'.reqWrites, j).Some?;
+        calc {
+          slice'[i];
+          dq'[j];
+          DiskQueue_JournalBlockAt(disk', j);
+          Queue_JournalBlockAt(disk'.reqWrites, j);
+          Some(JournalBlockGet(jr2, i - len));
+          slice_jr[i];
+        }
+      }
+    }
+    assert slice' == slice_jr;
+
+    calc {
+      concatFold(slice');
+      concatFold(slice_jr);
+      {
+        concatFoldAdditive(slice, mapSome(JournalBlocks(jr)));
+      }
+      JournalRangeConcat(concatFold(slice),
+            concatFold(mapSome(JournalBlocks(jr))));
+      {
+        concatFold_mapSome_JournalBlocks_eq_self(jr);
+      }
+      JournalRangeConcat(concatFold(slice), jr);
+    }
+
+    parseJournalRangeAdditive(concatFold(slice), jr);
+  }
 
   lemma DiskQueue_Journal_ProcessWrite(
       k: DiskConstants, disk: DiskState, disk': DiskState,
@@ -194,10 +530,68 @@ module JournalDiskUtils {
       id: ReqId)
   requires WFRange(start, len)
   requires AsyncSectorDisk.ProcessWrite(k, disk, disk', id)
+  requires ValidLocation(disk.reqWrites[id].loc);
   requires DiskQueue_HasJournal(disk, start, len)
   ensures DiskQueue_HasJournal(disk', start, len)
   ensures DiskQueue_Journal(disk', start, len)
        == DiskQueue_Journal(disk, start, len)
+  {
+    var dq := DiskQueue_JournalBlockSeq(disk);
+    var dq' := DiskQueue_JournalBlockSeq(disk');
+
+    var slice := CyclicSlice(dq, start, len);
+    var slice' := CyclicSlice(dq', start, len);
+
+    assert |slice'| == |slice|;
+    forall i | 0 <= i < |slice'| ensures slice'[i] == slice[i]
+    {
+      var j := JournalPosAdd(start, i);
+      calc {
+        slice[i];
+        dq[j];
+        DiskQueue_JournalBlockAt(disk, j);
+        {
+          var loc := JournalRangeLocation(j as uint64, 1);
+          if overlap(loc, disk.reqWrites[id].loc) {
+            journalLength1OverlapImpliesContained(
+                j as uint64, disk.reqWrites[id].loc);
+          }
+
+          /*
+          if (Queue_JournalBlockAt(disk.reqWrites, j).Some?) {
+            if (Queue_JournalBlockAt(disk'.reqWrites, j).None?) {
+              assert DiskQueue_JournalBlockAt(disk, j)
+                  == DiskQueue_JournalBlockAt(disk', j);
+            } else {
+              assert DiskQueue_JournalBlockAt(disk, j)
+                  == DiskQueue_JournalBlockAt(disk', j);
+            }
+          } else {
+            if (Queue_JournalBlockAt(disk'.reqWrites, j).None?) {
+              assert loc != disk.reqWrites[id].loc;
+              if overlap(loc, disk.reqWrites[id].loc) {
+                journalLength1OverlapImpliesContained(
+                    j as uint64, disk.reqWrites[id].loc);
+                assert false;
+              }
+              assert DiskQueue_JournalBlockAt(disk, j)
+                  == Disk_JournalBlockAt(disk.blocks, j)
+                  == Disk_JournalBlockAt(disk'.blocks, j)
+                  == DiskQueue_JournalBlockAt(disk', j);
+            } else {
+              assert DiskQueue_JournalBlockAt(disk, j)
+                  == DiskQueue_JournalBlockAt(disk', j);
+            }
+          }
+          */
+        }
+        DiskQueue_JournalBlockAt(disk', j);
+        dq'[j];
+        slice'[i];
+      }
+    }
+    assert slice' == slice;
+  }
 
   lemma Disk_Journal_ProcessWrite(
       k: DiskConstants, disk: DiskState, disk': DiskState,
@@ -211,4 +605,147 @@ module JournalDiskUtils {
   ensures Disk_HasJournal(disk'.blocks, start, len)
   ensures Disk_Journal(disk'.blocks, start, len)
        == Disk_Journal(disk.blocks, start, len)
+  {
+    var d := Disk_JournalBlockSeq(disk.blocks);
+    var d' := Disk_JournalBlockSeq(disk'.blocks);
+
+    var slice := CyclicSlice(d, start, len);
+    var slice' := CyclicSlice(d', start, len);
+
+    assert |slice'| == |slice|;
+    forall i | 0 <= i < |slice'| ensures slice'[i] == slice[i]
+    {
+      var j := JournalPosAdd(start, i);
+      var loc := JournalRangeLocation(j as uint64, 1);
+      assert !overlap(loc, disk.reqWrites[id].loc);
+      assert slice[i].Some?;
+      assert Disk_JournalBlockAtLoc(disk.blocks, loc).Some?;
+      assert loc in disk.blocks;
+      assert loc in disk'.blocks;
+      assert disk'.blocks[loc] == disk.blocks[loc];
+      calc {
+        slice[i];
+        d[j];
+        Disk_JournalBlockAt(disk.blocks, j);
+        Disk_JournalBlockAtLoc(disk.blocks, loc);
+        Disk_JournalBlockAtLoc(disk'.blocks, loc);
+        Disk_JournalBlockAt(disk'.blocks, j);
+        {
+          assert d'[j] == Disk_JournalBlockAt(disk'.blocks, j);
+        }
+        d'[j];
+        slice'[i];
+      }
+    }
+    assert slice' == slice;
+  }
+
+  lemma Disk_JournalRange_Read1(
+      disk: DiskState, start: int, len: int)
+  requires WFRange(start, len)
+  requires 1 <= len
+  requires start + len <= NumJournalBlocks() as int
+  requires Disk_HasJournalRange(disk.blocks, start, len)
+  requires ClosedUnderLogConcatenation(disk.blocks)
+  ensures JournalRangeLocation(start as uint64, len as uint64) in disk.blocks
+  ensures disk.blocks[JournalRangeLocation(start as uint64, len as uint64)].SectorJournal?
+  ensures Disk_JournalRange(disk.blocks, start, len)
+      == disk.blocks[JournalRangeLocation(start as uint64, len as uint64)].journal
+  {
+    if len == 1 {
+      var slice := CyclicSlice(Disk_JournalBlockSeq(disk.blocks), start, len);
+      assert slice[0].Some?;
+      assert Disk_JournalBlockSeq(disk.blocks)[start]
+          == Disk_JournalBlockAt(disk.blocks, start);
+      assert slice[0] == Disk_JournalBlockAt(disk.blocks, start);
+      JournalRangeConcatEmpty'(slice[0].value);
+      assert concatFold(slice)
+          == JournalRangeConcat(JournalRangeEmpty(), slice[0].value)
+          == slice[0].value;
+    } else {
+      var slice := CyclicSlice(Disk_JournalBlockSeq(disk.blocks), start, len);
+      var slice1 := CyclicSlice(Disk_JournalBlockSeq(disk.blocks), start, len-1);
+      assert slice1 == DropLast(slice);
+      Disk_JournalRange_Read1(disk, start, len-1);
+
+      var loc1 := JournalRangeLocation(start as uint64, len as uint64 - 1);
+      var loc2 := JournalRangeLocation(start as uint64 + len as uint64 - 1, 1);
+      var loc3 := JournalRangeLocation(start as uint64, len as uint64);
+      assert ClosedUnderLogConcatenationLocs(
+          disk.blocks, loc1, loc2, loc3);
+
+      assert slice[len - 1].Some?;
+
+      assert loc1 in disk.blocks;
+      assert loc2 in disk.blocks;
+      assert disk.blocks[loc1].SectorJournal?;
+      assert disk.blocks[loc2].SectorJournal?;
+      assert loc2.addr as int == loc1.addr as int + loc1.len as int;
+      assert loc3.addr == loc1.addr;
+      assert loc3.len as int == loc1.len as int + loc2.len as int;
+      assert loc3 in disk.blocks;
+    }
+  }
+
+  lemma Disk_JournalRange_Read2(
+      disk: DiskState, start: int, len: int)
+  requires WFRange(start, len)
+  requires 1 <= len
+  requires start + len > NumJournalBlocks() as int
+  requires Disk_HasJournalRange(disk.blocks, start, len)
+  requires ClosedUnderLogConcatenation(disk.blocks)
+  ensures JournalRangeLocation(start as uint64, NumJournalBlocks() - start as uint64) in disk.blocks
+  ensures disk.blocks[JournalRangeLocation(start as uint64, NumJournalBlocks() - start as uint64)].SectorJournal?
+  ensures JournalRangeLocation(0, len as uint64 - (NumJournalBlocks() - start as uint64)) in disk.blocks
+  ensures disk.blocks[JournalRangeLocation(0, len as uint64 - (NumJournalBlocks() - start as uint64))].SectorJournal?
+  ensures Disk_JournalRange(disk.blocks, start, len)
+      == JournalRangeConcat(
+        disk.blocks[JournalRangeLocation(start as uint64, NumJournalBlocks() - start as uint64)].journal,
+        disk.blocks[JournalRangeLocation(0, len as uint64 - (NumJournalBlocks() - start as uint64))].journal)
+  {
+    var slice := CyclicSlice(Disk_JournalBlockSeq(disk.blocks), start, len);
+    var slice1 := CyclicSlice(Disk_JournalBlockSeq(disk.blocks), start, NumJournalBlocks() as int - start);
+    var slice2 := CyclicSlice(Disk_JournalBlockSeq(disk.blocks), 0, len - (NumJournalBlocks() as int - start));
+    assert slice == slice1 + slice2;
+    assert slice1 == slice[.. NumJournalBlocks() as int - start];
+    assert slice2 == slice[NumJournalBlocks() as int - start ..];
+
+    Disk_JournalRange_Read1(disk, start, NumJournalBlocks() as int - start);
+    Disk_JournalRange_Read1(disk, 0, len - (NumJournalBlocks() as int - start));
+
+    concatFoldAdditive(slice1, slice2);
+  }
+
+  lemma Disk_Journal_Read1(
+      disk: DiskState, start: int, len: int)
+  requires WFRange(start, len)
+  requires 1 <= len
+  requires start + len <= NumJournalBlocks() as int
+  requires Disk_HasJournal(disk.blocks, start, len)
+  ensures JournalRangeLocation(start as uint64, len as uint64) in disk.blocks
+  ensures disk.blocks[JournalRangeLocation(start as uint64, len as uint64)].SectorJournal?
+  ensures Some(Disk_Journal(disk.blocks, start, len))
+      == parseJournalRange(disk.blocks[JournalRangeLocation(start as uint64, len as uint64)].journal)
+  {
+    Disk_JournalRange_Read1(disk, start, len);
+  }
+
+  lemma Disk_Journal_Read2(
+      disk: DiskState, start: int, len: int)
+  requires WFRange(start, len)
+  requires 1 <= len
+  requires start + len > NumJournalBlocks() as int
+  requires Disk_HasJournal(disk.blocks, start, len)
+  requires ClosedUnderLogConcatenation(disk.blocks)
+  ensures JournalRangeLocation(start as uint64, NumJournalBlocks() - start as uint64) in disk.blocks
+  ensures disk.blocks[JournalRangeLocation(start as uint64, NumJournalBlocks() - start as uint64)].SectorJournal?
+  ensures JournalRangeLocation(0, len as uint64 - (NumJournalBlocks() - start as uint64)) in disk.blocks
+  ensures disk.blocks[JournalRangeLocation(0, len as uint64 - (NumJournalBlocks() - start as uint64))].SectorJournal?
+  ensures Some(Disk_Journal(disk.blocks, start, len))
+      == parseJournalRange(JournalRangeConcat(
+        disk.blocks[JournalRangeLocation(start as uint64, NumJournalBlocks() - start as uint64)].journal,
+        disk.blocks[JournalRangeLocation(0, len as uint64 - (NumJournalBlocks() - start as uint64))].journal))
+  {
+    Disk_JournalRange_Read2(disk, start, len);
+  }
 }
